{
 "cells": [
  {
   "cell_type": "markdown",
   "metadata": {},
   "source": [
    "## Precision\n",
    "\n",
    "To derive the correlation matrices I am assuming a discrete time series of random values. I expect that the derivation in continuous time will proceed analogously.\n",
    "\n",
    "Assume $x$ is a stationary stochastic process. Then we can define:\n",
    "\n",
    "\\begin{align*}\n",
    "E(\\bar{x}) = \\mu &= \\frac{1}{n} \\sum_{i=1}^{n}{x_i} \\\\\n",
    "V(x) = \\sigma^2 = 1/\\pi &= \\frac{1}{n} \\sum_{i=1}^{n-h}{(x_i - \\bar{x})(x_i -\\bar{x})} \\\\\n",
    "C(x_n,x_{n+h}) = \\nu(h) &= \\frac{1}{n} \\sum_{i=1}^{n-h}{(x_i - \\bar{x})(x_{i+h} - \\bar{x})} \\\\\n",
    "\\rho(h) = \\nu(h)/\\sigma^2 &= \\pi \\nu(h) \\\\\n",
    "\\end{align*}\n",
    "\n",
    "where $\\mu$ is the mean, $\\sigma^2$ is the variance, $\\pi$ is the precision, $\\nu(h)$ is the cross-covariance, and $\\rho(h)$ is the autocorrelation function, with $\\rho(0) = 1$ by definition, when $n \\to \\infty$.\n",
    "\n",
    "Without loss of generality, we can assume $x$ is a zero mean process so we can simplify to:\n",
    "\n",
    "\\begin{align*}\n",
    "\\mu &= 0 \\\\\n",
    "\\sigma^2 = 1/\\pi &= \\frac{1}{n} \\sum_{i=1}^{n-h}{x_i x_i} \\\\\n",
    "\\nu(h) &= \\frac{1}{n} \\sum_{i=1}^{n-h}{x_i x_{i+h}} \\\\\n",
    "\\rho(h) &= \\pi \\nu(h) \\\\\n",
    "\\end{align*}\n",
    "\n",
    "If $x$ is not a single variable, but a set of variables, then the cross-covariance and precision of the process are matrices:\n",
    "\n",
    "\\begin{align*}\n",
    "\\Sigma^2 = \\Pi^{-1} = \\frac{1}{n} \\sum_{i=1}^{n-h}{x_i x_i^T} \\\\\n",
    "\\end{align*}\n",
    "\n",
    "If $\\tilde x$ is a vector of generalised coordinates, we have:\n",
    "\n",
    "\\begin{align*}\n",
    "\\tilde x &= [x, \\dot x, \\ddot x, \\dddot x, \\cdots]^T \\\\\n",
    "\\Sigma^2 &= \\frac{1}{n} \\sum_{i=1}^{n-h}{\\tilde x_i \\tilde x_i^T} \\\\\n",
    "&= \n",
    "    \\begin{bmatrix}\n",
    "    C(x,x) & C(x,\\dot{x}) & C(x,\\ddot{x}) & \\cdots \\\\\n",
    "    C(\\dot{x},x) & C(\\dot{x},\\dot{x}) & C(\\dot{x},\\ddot{x}) \\\\\n",
    "    C(\\ddot{x},x) & C(\\ddot{x},\\dot{x}) & C(\\ddot{x},\\ddot{x}) \\\\\n",
    "    \\vdots & & & \\ddots\n",
    "    \\end{bmatrix}\n",
    "\\end{align*}\n",
    "\n",
    "Because the levels in generalised coordinates are derivatives of the levels above, temporal correlations will exist between the levels. We can define the temporal derivative $x$:\n",
    "\n",
    "\\begin{align*}\n",
    "\\lim_{\\Delta t \\to 0} E \\left( \\dot{x}(t) - \\frac{x(t + \\Delta t) - x(t)}{\\Delta t}\\right) = 0 \\\\\n",
    "\\end{align*}\n",
    "\n",
    "or, more informally, using the finite difference method:\n",
    "\n",
    "\\begin{align*}\n",
    "\\dot{x}(t) &= \\frac{x(t + \\Delta t) - x(t)}{\\Delta t} ; \\Delta t \\to 0\\\\\n",
    "\\ddot{x}(t) &= \\frac{\\dot{x}(t + \\Delta t) - \\dot{x}(t)}{\\Delta t} \\\\\n",
    "&= \\frac{x(t + \\Delta t) - x(t)}{(\\Delta t)^2} - \\frac{x(t) - x(t - \\Delta t)}{(\\Delta t)^2}\\\\\n",
    "&= \\frac{x(t + \\Delta t) - 2x(t) + x(t - \\Delta t)}{(\\Delta t)^2}; \\Delta t \\to 0\\\\\n",
    "\\end{align*}"
   ]
  },
  {
   "cell_type": "markdown",
   "metadata": {},
   "source": [
    "Thus, we can proceed as follows:\n",
    "\n",
    "\\begin{align*}\n",
    "C(x,x) &= \\sigma^2 \\rho(0)\\\\\n",
    "\\\\\n",
    "C(x,\\dot{x}) &= \\frac{1}{n} \\sum_{i=1}^{n}{x_i \\dot{x}_i} \\\\\n",
    "&= \\frac{1}{n} \\sum_{i=1}^{n}{x(i) \\frac{x(i + \\Delta t) - x(i)}{\\Delta t}} \\\\\n",
    "&= \\frac{1}{n} \\sum_{i=1}^{n}{\\frac{x(i) x(i + \\Delta t) - x(i) x(i)}{\\Delta t}} \\\\\n",
    "&= \\frac{\\nu(\\Delta t) - \\nu(0)}{\\Delta t} \\\\\n",
    "&= \\dot{\\nu}(0) \\\\\n",
    "&= \\sigma^2\\dot{\\rho}(0) \\\\\n",
    "\\\\\n",
    "C(x,\\ddot{x}) &= \\frac{1}{n} \\sum_{i=1}^{n}{x(i) \\frac{x(i + \\Delta t) - 2x(i) + x(i - \\Delta t)}{(\\Delta t)^2}} \\\\\n",
    "&= \\frac{1}{n} \\sum_{i=1}^{n}{\\frac{x(i) x(i + \\Delta t) - 2x(i) x(i) + x(i) x(i - \\Delta t)}{(\\Delta t)^2}} \\\\\n",
    "&= \\frac{\\nu(\\Delta t) - 2\\nu(0) + \\nu(- \\Delta t)}{(\\Delta t)^2} \\\\\n",
    "&= \\sigma^2 \\frac{\\dot{\\rho}(\\Delta t) - \\dot{\\rho}(0)}{\\Delta t} \\\\\n",
    "&= \\sigma^2 \\ddot{\\rho}(0) \\\\\n",
    "\\\\\n",
    "C(x,\\dddot{x}) &= \\frac{1}{n} \\sum_{i=1}^{n}x(i) \\frac{x(t + 2\\Delta t) - 3x(t + \\Delta t) + 3x(t) - x(t - \\Delta t)}{(\\Delta t)^3} \\\\\n",
    "&= \\frac{1}{n} \\sum_{i=1}^{n} \\frac{x(i)x(t + 2\\Delta t) - 3x(i)x(t + \\Delta t) + 3x(i)x(t) - x(i)x(t - \\Delta t)}{(\\Delta t)^3} \\\\\n",
    "&= \\frac{\\nu(2\\Delta t) - 3\\nu(\\Delta t) + 3\\nu(0) - \\nu( - \\Delta t)}{(\\Delta t)^3} \\\\\n",
    "&= \\sigma^2 \\dddot{\\rho}(0) \\\\\n",
    "\\\\\n",
    "C(x,\\ddot{\\ddot{x}}) &= \\frac{1}{n} \\sum_{i=1}^{n}{x_i \\ddot{\\ddot{x}}_i} \\\\\n",
    "&= \\frac{1}{n} \\sum_{i=1}^{n}{x(i) \\frac{x(i + 2\\Delta t) - 4x(i + \\Delta t) + 6x(i) - 4x(i - \\Delta t) + x(i - 2\\Delta t)}{\\Delta t^4}} \\\\\n",
    "&= \\frac{1}{n} \\sum_{i=1}^{n}{\\frac{x(i)x(i + 2\\Delta t) - 4x(i)x(i + \\Delta t) + 6x(i)^2 - 4x(i)x(i - \\Delta t) + x(i)(x(i - 2\\Delta t)}{\\Delta t^4}} \\\\\n",
    "&= \\frac{\\nu(2\\Delta t) - 4\\nu(\\Delta t) + 6\\nu(0) - 4\\nu(-\\Delta t) + \\nu(-2\\Delta t)}{\\Delta t^4}\\\\\n",
    "&= \\ddot{\\ddot{\\nu}}(0)\\\\\n",
    "&= \\sigma^2 \\ddot{\\ddot{\\rho}}(0)\\\\\n",
    "\\\\\n",
    "C(\\dot{x},\\dot{x}) &= \\frac{1}{n} \\sum_{i=1}^{n}{\\dot{x}_i \\dot{x}_i} \\\\\n",
    "&= \\frac{1}{n} \\sum_{i=1}^{n}{\\frac{x(i + \\Delta t) - x(i)}{\\Delta t} \\frac{x(i + \\Delta t) - x(i)}{\\Delta t}} \\\\\n",
    "&= \\frac{1}{n} \\sum_{i=1}^{n}{\\frac{x(i + \\Delta t) x(i + \\Delta t) - 2x(i) x(i + \\Delta t) + x(i)x(i)}{(\\Delta t)^2}} \\\\\n",
    "&= \\frac{2\\nu(0) - 2\\nu(\\Delta t)}{(\\Delta t)^2} \\\\\n",
    "&= \\frac{-\\nu(\\Delta t) + 2\\nu(0) - \\nu(-\\Delta t)}{(\\Delta t)^2} \\; \\text{since} \\; \\nu(i) = \\nu(-i)\\\\\n",
    "&= -\\ddot{\\nu}(0)\\\\\n",
    "&= -\\sigma^2 \\ddot{\\rho}(0)\\\\\n",
    "\\\\\n",
    "C(\\dot{x},\\ddot{x}) &= \\frac{1}{n} \\sum_{i=1}^{n}{\\dot{x}_i \\ddot{x}_i} \\\\\n",
    "&= \\frac{1}{n} \\sum_{i=1}^{n}{\\frac{x(i + \\Delta t) - x(i)}{\\Delta t} \\frac{x(i + \\Delta t) - 2x(i) + x(i - \\Delta t)}{\\Delta t^2}} \\\\\n",
    "&= \\frac{1}{n} \\sum_{i=1}^{n}{\\frac{x(i + \\Delta t)x(i + \\Delta t) - 2x(i + \\Delta t)x(i) + x(i + \\Delta t)x(i - \\Delta t) - x(i)x(i + \\Delta t) + 2x(i)x(i) - x(i)x(i - \\Delta t)}{\\Delta t^3}} \\\\\n",
    "&= \\frac{\\nu(0) - 2\\nu(\\Delta t) + \\nu(2\\Delta t) - \\nu(\\Delta t) + 2\\nu(0) - \\nu(\\Delta t)}{\\Delta t^3} \\\\\n",
    "&= \\frac{3\\nu(0) - 4\\nu(\\Delta t) + \\nu(2\\Delta t)}{\\Delta t^3} \\\\\n",
    "&= \\frac{\\nu(2\\Delta t) - 3\\nu(\\Delta t) + 3\\nu(0) - \\nu(-\\Delta t)}{\\Delta t^3} \\\\\n",
    "&= \\dddot{\\nu}(0)\\\\\n",
    "&= \\sigma^2 \\dddot{\\rho}(0)\\\\\n",
    "\\\\\n",
    "C(\\dot{x},\\dddot{x}) &= \\frac{1}{n} \\sum_{i=1}^{n}{\\dot{x}_i \\dddot{x}_i} \\\\\n",
    "&= \\frac{1}{n} \\sum_{i=1}^{n}{\\frac{x(i + \\Delta t) - x(i)}{\\Delta t} \\frac{x(i + 2\\Delta t) - 3x(i + \\Delta t) + 3x(i) - x(i - \\Delta t)}{\\Delta t^3}} \\\\\n",
    "&= \\frac{1}{n} \\sum_{i=1}^{n}{\\frac{x(i + \\Delta t)x(i + 2\\Delta t) - 3x(i + \\Delta t)^2 + 3x(i + \\Delta t)x(i) - x(i + \\Delta t)x(i - \\Delta t) }{\\Delta t^4}} \\\\\n",
    "&- \\frac{1}{n} \\sum_{i=1}^{n}{\\frac{x(i)x(i + 2\\Delta t) - 3x(i)x(i + \\Delta t) + 3x(i)^2 - x(i)x(i - \\Delta t)}{\\Delta t^4}} \\\\\n",
    "&= \\frac{\\nu(\\Delta t) - 3\\nu(0) + 3\\nu(\\Delta t) - \\nu(2\\Delta t) - \\nu(2\\Delta t) + 3\\nu(\\Delta t) - 3\\nu(0) + \\nu(\\Delta t)}{\\Delta t^4}\\\\\n",
    "&= \\frac{8\\nu(\\Delta t) - 6 \\nu(0) - 2\\nu(2\\Delta t)}{\\Delta t^4} \\\\\n",
    "&= -\\frac{\\nu(2\\Delta t) - 4\\nu(\\Delta t) + 6\\nu(0) - 4\\nu(-\\Delta t) + \\nu(-2\\Delta t)}{\\Delta t^4} \\\\\n",
    "&= - \\ddot{\\ddot{\\nu}}(0) \\\\\n",
    "&= -\\sigma^2 \\ddot{\\ddot{\\rho}}(0)\\\\\n",
    "\\\\\n",
    "C(\\dot{x},\\ddot{\\ddot{x}}) &= \\frac{1}{n} \\sum_{i=1}^{n}{\\dot{x}_i \\ddot{\\ddot{x}}_i} \\\\\n",
    "&= \\frac{1}{n} \\sum_{i=1}^{n}{\\frac{x(i + \\Delta t) - x(i)}{\\Delta t} \\frac{x(i + 2\\Delta t) - 4x(i + \\Delta t) + 6x(i) - 4x(i - \\Delta t) + x(i - 2\\Delta t)}{\\Delta t^4}} \\\\\n",
    "&= \\frac{1}{n} \\sum_{i=1}^{n}{\\frac{x(i + \\Delta t)x(i + 2\\Delta t) - 4x(i + \\Delta t)^2 + 6x(i + \\Delta t)x(i) - 4x(i + \\Delta t)x(i - \\Delta t) + x(i + \\Delta t)x(i - 2\\Delta t) }{\\Delta t^5}} \\\\\n",
    "&- \\frac{1}{n} \\sum_{i=1}^{n}{\\frac{x(i)x(i + 2\\Delta t) - 4x(i)x(i + \\Delta t) + 6x(i)^2 - 4x(i)x(i - \\Delta t) + x(i)(x(i - 2\\Delta t)}{\\Delta t^5}} \\\\\n",
    "&= \\frac{\\nu(\\Delta t) - 4\\nu(0) + 6\\nu(\\Delta t) - 4\\nu(2\\Delta t) + \\nu(3\\Delta t)- \\nu(2\\Delta t) + 4\\nu(\\Delta t) - 6\\nu(0) + 4\\nu(\\Delta t) - \\nu(2\\Delta t)}{\\Delta t^5}\\\\\n",
    "&= \\frac{\\nu(3\\Delta t) - 6\\nu(2\\Delta t) + 15\\nu(\\Delta t) - 10 \\nu(0) }{\\Delta t^5} \\\\\n",
    "&= \\frac{\\nu(3\\Delta t) - 5\\nu(2\\Delta t) + 10\\nu(\\Delta t) - 10 \\nu(0) + 5\\nu(-\\Delta t) - \\nu(-2\\Delta t)}{\\Delta t^5} \\\\\n",
    "&= \\ddot{\\dddot{\\nu}}(0)\\\\\n",
    "&= \\sigma^2 \\ddot{\\dddot{\\rho}}(0)\\\\\n",
    "\\\\\n",
    "C(\\ddot{x},\\ddot{x}) &= \\frac{1}{n} \\sum_{i=1}^{n}{\\ddot{x}_i \\ddot{x}_i} \\\\\n",
    "&= \\frac{1}{n} \\sum_{i=1}^{n}{\\frac{x(i + \\Delta t) - 2x(i) + x(i - \\Delta t)}{\\Delta t^2} \\frac{x(i + \\Delta t) - 2x(i) + x(i - \\Delta t)}{\\Delta t^2}} \\\\\n",
    "&= \\frac{1}{n} \\sum_{i=1}^{n}{\\frac{x(i + \\Delta t)x(i + \\Delta t) - 2x(i)x(i + \\Delta t) + x(i + \\Delta t)x(i - \\Delta t) }{\\Delta t^4}} \\\\\n",
    "&- \\frac{1}{n} \\sum_{i=1}^{n}{\\frac{2x(i)x(i + \\Delta t) - 4x(i)x(i) + 2x(i)x(i - \\Delta t) }{\\Delta t^4}} \\\\\n",
    "&+ \\frac{1}{n} \\sum_{i=1}^{n}{\\frac{x(i - \\Delta t)x(i + \\Delta t) - 2x(i - \\Delta t)x(i) + x(i - \\Delta t)x(i - \\Delta t)}{\\Delta t^4}} \\\\\n",
    "&= \\frac{\\nu(0) - 2\\nu(\\Delta t) + \\nu(2\\Delta t) - 2\\nu(\\Delta t) + 4\\nu(0) - 2\\nu(\\Delta t) + \\nu(2\\Delta t) - 2\\nu(\\Delta t) + \\nu(0)}{\\Delta t^4} \\\\\n",
    "&= \\frac{6\\nu(0) - 8\\nu(\\Delta t) + 2\\nu(2\\Delta t)}{\\Delta t^4} \\\\\n",
    "&= \\frac{\\nu(2\\Delta t) - 4\\nu(\\Delta t) + 6\\nu(0) - 4\\nu(-\\Delta t) + \\nu(-2\\Delta t)}{\\Delta t^4} \\\\\n",
    "&= \\ddot{\\ddot{\\nu}}(0) \\\\\n",
    "&= \\sigma^2 \\ddot{\\ddot{\\rho}}(0)\\\\\n",
    "\\\\\n",
    "C(\\ddot{x},\\dddot{x}) &= \\frac{1}{n} \\sum_{i=1}^{n}{\\ddot{x}_i \\dddot{x}_i} \\\\\n",
    "&= \\frac{1}{n} \\sum_{i=1}^{n}{\\frac{x(i + \\Delta t) - 2x(i) + x(i - \\Delta t)}{\\Delta t^2} \\frac{x(i + 2\\Delta t) - 3x(i + \\Delta t) + 3x(i) - x(i - \\Delta t)}{\\Delta t^3}} \\\\\n",
    "&= \\frac{1}{n} \\sum_{i=1}^{n}{\\frac{x(i + \\Delta t)x(i + 2\\Delta t) - 3x(i + \\Delta t)x(i + \\Delta t) + 3x(i + \\Delta t)x(i) - x(i + \\Delta t)x(i - \\Delta t) }{\\Delta t^5}} \\\\\n",
    "&- \\frac{1}{n} \\sum_{i=1}^{n}{\\frac{2x(i)x(i + 2\\Delta t) - 6x(i)x(i + \\Delta t) + 6x(i)x(i) - x(i)x(i - \\Delta t) }{\\Delta t^5}} \\\\\n",
    "&+ \\frac{1}{n} \\sum_{i=1}^{n}{\\frac{x(i - \\Delta t)x(i + 2\\Delta t) - 3x(i - \\Delta t)x(i + \\Delta t) + 3x(i - \\Delta t)x(i) - x(i - \\Delta t)x(i - \\Delta t) }{\\Delta t^5}} \\\\\n",
    "&= \\frac{\\nu(3\\Delta t) - 6 \\nu(2\\Delta t) + 15\\nu(\\Delta t) - 10\\nu(0)  }{\\Delta t^5} \\\\\n",
    "&= \\frac{\\nu(3\\Delta t) - 5 \\nu(2\\Delta t) + 10\\nu(\\Delta t) - 10\\nu(0) + 5\\nu(-\\Delta t) - \\nu(-2\\Delta t)}{\\Delta t^5} \\\\\n",
    "&= \\ddot{\\dddot{\\nu}}(0)\\\\\n",
    "&= \\sigma^2 \\ddot{\\dddot{\\rho}}(0)\n",
    "\\end{align*}\n",
    "\n",
    "The pattern emerging is that the correlation between derivatives of order $j$ and $k$ yields the $j+k$'s derivative of the autocorrelation function multiplied by $\\sigma^2$ and by $-1$ if both $j$ and $k$ are odd."
   ]
  },
  {
   "cell_type": "markdown",
   "metadata": {},
   "source": [
    "## Autocorrelation function\n",
    "\n",
    "The autocorrelation function $\\rho(h)$ for a given delay $h$ is symmetric around $h=0$. In other words, $\\rho$ is an even function. This implies directly that $\\dot{\\rho}(h)$ is odd, $\\ddot{\\rho}(h)$ is even, etc. Odd functions evaluated at $0$ yield $0$. Also $\\rho(0) = 1$ by construction. Thus we can simplyfy $S$ as:\n",
    "\n",
    "\\begin{align*}\n",
    "S =\n",
    "    \\begin{bmatrix}\n",
    "    1 & 0 & \\ddot{\\rho}(0) & 0 & \\ddot{\\ddot{\\rho}}(0) & 0 & \\cdots \\\\\n",
    "    0 & -\\ddot{\\rho}(0) & 0 & -\\ddot{\\ddot{\\rho}}(0) & 0 & -\\dddot{\\dddot{\\rho}}(0)\\\\\n",
    "    \\ddot{\\rho}(0) & 0 & \\ddot{\\ddot{\\rho}}(0) & 0 & \\dddot{\\dddot{\\rho}}(0) & 0 \\\\\n",
    "    0 & -\\ddot{\\ddot{\\rho}}(0) & 0 & -\\dddot{\\dddot{\\rho}}(0) & 0 & -\\ddot{\\dddot{\\dddot{\\rho}}}(0) \\\\\n",
    "    \\ddot{\\ddot{\\rho}}(0) & 0 & \\dddot{\\dddot{\\rho}}(0) & 0 & \\ddot{\\dddot{\\dddot{\\rho}}}(0) & 0 \\\\\n",
    "    0 & -\\dddot{\\dddot{\\rho}}(0) & 0 & -\\ddot{\\dddot{\\dddot{\\rho}}}(0) & 0 & -\\ddot{\\ddot{\\dddot{\\dddot{\\rho}}}}(0)\\\\\n",
    "    \\vdots & & & & & & \\ddots\n",
    "    \\end{bmatrix}^{-1}\n",
    "\\end{align*}\n",
    "\n",
    "$S$ can be evaluated for any analytic autocorrelation function. If we assume, for convenience, that the temporal correlation of all innovations have the same Gaussian form with precision parameter $\\gamma$, we can proceed with:\n",
    "\n",
    "\\begin{align*}\n",
    "\\rho(h) &= \\exp{-\\frac{\\gamma}{2} h^2} \\\\\n",
    "\\dot{\\rho}(h) &= -\\gamma h \\rho(h) \\\\\n",
    "\\ddot{\\rho}(h) &= -\\gamma \\rho(h) + (\\gamma h)^2 \\rho(h) \\\\\n",
    "\\dddot{\\rho}(h) &= \\gamma^2 h \\rho(h) + 2 \\gamma^2 h \\rho(h) - (\\gamma h)^3 \\rho(h) \\\\\n",
    "&= 3 \\gamma^2 h \\rho(h) - (\\gamma h)^3 \\rho(h) \\\\\n",
    "\\ddot{\\ddot{\\rho}}(h) &= 3 \\gamma^2 \\rho(h) - 3 \\gamma^3 h^2 \\rho(h) - 3 \\gamma^3 h^2 \\rho(h) + (\\gamma h)^4 \\rho(h) \\\\\n",
    "&= 3 \\gamma^2 \\rho(h) - 6 \\gamma^3 h^2 \\rho(h) + (\\gamma h)^4 \\rho(h) \\\\\n",
    "\\ddot{\\dddot{\\rho}}(h) &= - 3 \\gamma^3 h \\rho(h) - 12 \\gamma^3 h \\rho(h) + 6 \\gamma^4 h^3 \\rho(h) + 4 \\gamma^4 h^3 \\rho(h) - (\\gamma h)^5 \\rho(h) \\\\\n",
    "&= - 15 \\gamma^3 h \\rho(h) + 10 \\gamma^4 h^3 \\rho(h) - (\\gamma h)^5 \\rho(h) \\\\\n",
    "\\dddot{\\dddot{\\rho}}(h) &= -15 \\gamma^3 \\rho(h) + 15 \\gamma^4 h^2 \\rho(h) + 30 \\gamma^4 h^2 \\rho(h) - 10 \\gamma^5 h^4 \\rho(h) - 5 \\gamma^5 h^4 \\rho(h) + (\\gamma h)^6 \\rho(h) \\\\\n",
    "&= -15 \\gamma^3 \\rho(h) + 45 \\gamma^4 h^2 \\rho(h) - 15 \\gamma^5 h^4 \\rho(h) + (\\gamma h)^6 \\rho(h) \\\\\n",
    "\\end{align*}\n",
    "\n",
    "To calculate the higher order derivatives, the Hermite polynomials can be used as a shortcut to find the relevant coefficients.\n",
    "\n",
    "Evaluating the above at $h = 0$ yields:\n",
    "\n",
    "\\begin{align*}\n",
    "\\rho(0) &= 1 \\\\\n",
    "\\dot{\\rho}(0) &= 0 \\\\\n",
    "\\ddot{\\rho}(0) &= -\\gamma \\\\\n",
    "\\dddot{\\rho}(0) &= 0 \\\\\n",
    "\\ddot{\\ddot{\\rho}}(0) &= 3 \\gamma^2 \\\\\n",
    "\\ddot{\\dddot{\\rho}}(0) &= 0 \\\\\n",
    "\\dddot{\\dddot{\\rho}}(0) &= -15 \\gamma^3 \\\\\n",
    "\\end{align*}\n",
    "\n",
    "From the Hermite polynomials we can quickly find the coefficient for all even order derivatives of order $n$:\n",
    "\n",
    "\\begin{align*}\n",
    "c_n = n! \\frac{(-1)^{n/2}}{2^{n/2+1}(n/2)!}\n",
    "\\end{align*}\n",
    "\n"
   ]
  },
  {
   "cell_type": "code",
   "execution_count": 7,
   "metadata": {},
   "outputs": [
    {
     "name": "stdout",
     "output_type": "stream",
     "text": [
      "Derivatives of 𝜌\n",
      "0        1.0 γ^0\n",
      "1          0\n",
      "2       -1.0 γ^1\n",
      "3          0\n",
      "4        3.0 γ^2\n",
      "5          0\n",
      "6      -15.0 γ^3\n",
      "7          0\n",
      "8      105.0 γ^4\n",
      "9          0\n",
      "10    -945.0 γ^5\n",
      "11         0\n"
     ]
    }
   ],
   "source": [
    "from math import factorial as fac\n",
    "print(\"Derivatives of 𝜌\")\n",
    "for m in range(6):\n",
    "    print(\"{:<3} {:>8} γ^{:}\".format(2*m, (-1)**m * fac(2*m) / fac(m) / 2**(m), m))\n",
    "    print(\"{:<3} {:>8}\".format(2*m + 1, 0))"
   ]
  },
  {
   "cell_type": "markdown",
   "metadata": {},
   "source": [
    "\\begin{align*}\n",
    "S &=\n",
    "    \\begin{bmatrix}\n",
    "    1 & 0 & \\ddot{\\rho}(0) & 0 & \\ddot{\\ddot{\\rho}}(0) & 0  \\\\\n",
    "    0 & -\\ddot{\\rho}(0) & 0 & -\\ddot{\\ddot{\\rho}}(0) & 0 & -\\dddot{\\dddot{\\rho}}(0)\\\\\n",
    "    \\ddot{\\rho}(0) & 0 & \\ddot{\\ddot{\\rho}}(0) & 0 & \\dddot{\\dddot{\\rho}}(0) & 0 \\\\\n",
    "    0 & -\\ddot{\\ddot{\\rho}}(0) & 0 & -\\dddot{\\dddot{\\rho}}(0) & 0 & -\\ddot{\\dddot{\\dddot{\\rho}}}(0) \\\\\n",
    "    \\ddot{\\ddot{\\rho}}(0) & 0 & \\dddot{\\dddot{\\rho}}(0) & 0 & \\ddot{\\dddot{\\dddot{\\rho}}}(0) & 0 \\\\\n",
    "    0 & -\\dddot{\\dddot{\\rho}}(0) & 0 & -\\ddot{\\dddot{\\dddot{\\rho}}}(0) & 0 & -\\ddot{\\ddot{\\dddot{\\dddot{\\rho}}}}(0)\\\\\n",
    "    \\end{bmatrix}^{-1}\\\\\n",
    "&=\n",
    "    \\begin{bmatrix}\n",
    "    1 & 0 & -\\gamma & 0 & 3 \\gamma^2 & 0 \\\\\n",
    "    0 & \\gamma & 0 & -3 \\gamma^2 & 0 & 15 \\gamma^3 \\\\\n",
    "    -\\gamma & 0 & 3 \\gamma^2 & 0 & -15 \\gamma^3 & 0 \\\\\n",
    "    0 & -3 \\gamma^2 & 0 & 15 \\gamma^3 & 0 & -105 \\gamma^4 \\\\\n",
    "    3 \\gamma^2 & 0 & -15 \\gamma^3 & 0 & 105 \\gamma^4 & 0 \\\\\n",
    "    0 & 15 \\gamma^3 & 0 & -105 \\gamma^4 & 0 & 945 \\gamma^5 \\\\\n",
    "    \\end{bmatrix}^{-1}\n",
    "\\end{align*}\n",
    "\n",
    "So here the pattern arising is that the diagonal contains only positive coefficients, the diagonals shifted by 2 only negative coefficients, those by four only positive coefficients, etc.\n",
    "\n",
    "Note, to get Friston's version, we need to replace $\\gamma$ with $\\gamma / 2$. I'm not sure where this discrepancy comes from. It could just be a matter of how you define precision, but in that case his version would be odd, as it results in $\\rho(h) = \\exp(-\\gamma h^2/4)$. "
   ]
  }
 ],
 "metadata": {
  "kernelspec": {
   "display_name": "Python 3",
   "language": "python",
   "name": "python3"
  },
  "language_info": {
   "codemirror_mode": {
    "name": "ipython",
    "version": 3
   },
   "file_extension": ".py",
   "mimetype": "text/x-python",
   "name": "python",
   "nbconvert_exporter": "python",
   "pygments_lexer": "ipython3",
   "version": "3.7.5"
  }
 },
 "nbformat": 4,
 "nbformat_minor": 2
}
